[rp] Now, whenever a new term is added to the context, all of the context is attempted to be rewritten again. For example, if the context only has this entry: "(or (foo1 x) (foo2 x)" and we are currently rewriting a term "(if (foo1 x) then else)", then when we are writing the "then" branch, the context will only have "(foo1 x)"; and when we are rewriting the "else" branch, the context will only have "(foo2 x)". This system will make it easier to casesplit and help make the order of elements in the context irrelevant.

books/projects/rp-rewriter/aux-functions.lisp
@@ -697,8 +697,8 @@
         ((case-match term (('not &) t))
          (mv (acl2::fargn term 1) t))
         ((case-match term (('if & then ''nil) (nonnil-p then)))
-         (mv (acl2::fcons-term* 'not (acl2::fargn term 1))
-             `(nil t)))
+         (mv `(if ,(acl2::fargn term 1) 'nil 't)
+             `(nil t t t)))
         ((case-match term (('if & ''nil else) (nonnil-p else)))
          (mv (acl2::fargn term 1) t))
         ((and (case-match term (('equal & &) t))
@@ -711,7 +711,7 @@
                  (acl2::fargn term 1)
                (acl2::fargn term 2))
              t))
-        (t (mv (acl2::fcons-term* 'not term) `(nil t)))))
+        (t (mv `(if ,term 'nil 't) `(nil t t t)))))
 
 (encapsulate
   nil
@@ -1870,3 +1870,15 @@ In the hyps: ~p0, in the rhs :~p1. ~%")))|#
        (rp-state-preservedp-sk old-rp-state
                                new-rp-state)))     
        
+
+(define not* (x)
+  (not x)
+  ///
+  (defthm not*-forward
+    (implies (not* x)
+             (not x))
+    :rule-classes :forward-chaining)
+  (defthm not-of-not*-forward
+    (implies (not (not* a))
+             a)
+    :rule-classes :forward-chaining))
